format-version: 1.2

[Typedef]
id: has_external_link_to
name: has external link to
def: "an instance of the term must contain a link to an external
     resource of the specified type" []

[Typedef]
id: usually_has_external_link_to
name: usually has external link to
def: "an instance of the term should contain a link to an external
     resource of the specified type" []
comment: used when links of that type are generally available

[Typedef]
id: ideally_has_external_link_to
name: ideally has external link to
def: "ideally, an instance of the term contains a link to an external
     resource of the specified type" []
comment: used when links of that type are generally not available

[Typedef]
id: has_optional_type
name: has optional type
def: "instances of the subject term can be classified as of type O, where
     O is an instance of the object term, but this classication system
     does not apply in all cases" []

[Typedef]
id: defined_by
name: defined by
def: "instances of the subject term are defined by the mean
     of instances of the object term" []

[Term]
id: M0001
name: logical_expression
namespace: metadata
def: "an expression involving one or muliple terms, the set operators
     for intersection (and), union (or), and inversion (not)" []

[Term]
id: M0010
name: groups_logical_expression
namespace: metadata
def: "a logical expression whose terms are groups of organisms" []
comment: avoiding nested group combinations can simplify applications
is_a: M0001 ! logical_expression

[Term]
id: M0002
name: groups_combination_expression
namespace: metadata
def: "a combination of multiple organism groups, expressed in terms
     or a logical expression, combining two or more other groups" []
is_a: M0010 ! groups_logical_expression

[Term]
id: M0011
name: group_inversion_expression
namespace: metadata
def: "a group logical expression, containing only the negation symbol
     and a single term (group)" []
is_a: M0010 ! groups_logical_expression

[Term]
id: M0003
name: external_resource
namespace: metadata
def: "a source of definitions or information which is maintained
     and made available by third-parties" []
comment: only publicly available resources should be used

[Term]
id: M0004
name: external_definition
namespace: metadata
def: "a definition given in a document or database maintained and
     made available by third-parties" []
is_a: M0003 ! external_resource

[Term]
id: M0005
name: external_enumeration
namespace: metadata
def: "a list of members of a class, given in a document
     or database, maintained and made available by third-parties" []
is_a: M0003 ! external_resource

[Term]
id: M0006
name: taxonomy_database
namespace: metadata
def: "a database, which contain definitions of group of organisms
     by their biological taxonomic classification" []
is_a: M0003 ! external_resource

[Term]
id: M0007
name: strains_database
namespace: metadata
def: "a database, containing the names of strains, their availability
     in strain collections and other relevant information" []
is_a: M0003 ! external_resource

[Term]
id: M0008
name: NCBI_taxonomy_database
namespace: metadata
def: "the taxonomy database maintained by NCBI" []
is_a: M0006 ! taxonomy_database

[Term]
id: M0009
name: taxonomic_rank
namespace: metadata
def: "name of one of the hierarchical levels of a taxonomic classification" []
comment: example: species, genus, family; not all taxonomic group have a specific rank

[Term]
id: GC0001
name: group_types_category
namespace: hierarchy_root
def: "higher level definition, which includes one or multiple types of groups
     or biological organisms" []

[Term]
id: GC0002
name: habitat_requirement_type
namespace: group_types_category
def: "organisms classification by required conditions in their habitats" []
is_a: GC0001 ! group_types_category

[Term]
id: GC0003
name: phenotype_group_type
namespace: group_types_category
def: "groups of organisms by one particular aspect of their phenotype" []
comment: this does not include groups by characteristics of \
         the habitat such as temperature, salinity, pH, etc, \
         which are included instead in habitat_requirement_type (GC0002)
is_a: GC0001 ! group_types_category

[Term]
id: GC0004
name: location_group_type
namespace: group_types_category
def: "groups of organisms by the location where their live" []
is_a: GC0001 ! group_types_category

[Term]
id: GC0005
name: derived_group_type
namespace: group_types_category
def: "definition of groups of organisms derived by the definition of one or
     multiple other groups" []
is_a: GC0001 ! group_types_category

[Term]
id: GC0006
name: phylogenetic_group_type
namespace: group_types_category
def: "groups of organisms by a currently or historically inferred
     phylogenetic relationship" []
is_a: GC0001 ! group_types_category

[Term]
id: GG0001
name: taxonomic
namespace: group_type
def: "organisms belonging to a group with common phylogenetic origin,
     as defined by an official taxonomy organisation or by
     a commonly used taxonomy database" []
comment: ideally represents a monophiletic group or organisms, a clade
relationship: has_external_link_to M0006 ! taxonomy_database
  comment: recommended: M0008 ! NCBI_taxonomy_database
relationship: has_optional_type M0009 ! taxonomic_rank
is_a: GC0006 ! phylogenetic_group_type

[Term]
id: GG0002
name: strain
namespace: group_type
def: "prokaryotic organisms which were cultivated in a biological laboratory
     starting from a common ancestor" []
comment: may be assigned or not to a specific taxonomic group; it should \
         be linked to NCBI taxonomy, if the strain itself is included there; to \
         the species, if the strain is assigned to a species, but not included \
         in NCBI taxonomy; to the genus, if the strain is not included in NCBI \
         taxonomy and not assigned to a species, but assigned to a genus
relationship: usually_has_external_link_to M0008 ! NCBI_taxonomy_database
relationship: usually_has_external_link_to M0007 ! strains_database
is_a: GC0006 ! phylogenetic_group_type

[Term]
id: GG0004
name: metagenomic_assembled
namespace: group_type
def: "organism known only because its genome was assembled from a metagenome" []
comment: may be assigned or not to a specific taxonomic group; it should \
         be linked to NCBI taxonomy, if the strain itself is included there; to \
         the species, if the strain is assigned to a species, but not included \
         in NCBI taxonomy; to the genus, if the strain is not included in NCBI \
         taxonomy and not assigned to a species, but assigned to a genus
relationship: usually_has_external_link_to M0008 ! NCBI_taxonomy_database
relationship: usually_has_external_link_to M0007 ! strains_database
is_a: GC0006 ! location

[Term]
id: GG0003
name: paraphyletic
namespace: group_type
def: "named group of strains or species or other taxa, which which do not
     represent a monophyetic group" []
comment: usually historically a taxonomic group, but not recognized anymore as such
relationship: usually_has_external_link_to M0004 ! external_definition
relationship: ideally_has_external_link_to M0005 ! external_enumeration
is_a: GC0006 ! phylogenetic_group_type

[Term]
id: GL0001
name: geographical
namespace: group_type
def: "organisms living in a specific named geographical area,
     of any kind and size" []
relationship: usually_has_external_link_to M0004 ! external_definition
relationship: ideally_has_external_link_to M0005 ! external_enumeration
is_a: GC0004 ! location_group_type

[Term]
id: GL0002
name: habitat
namespace: group_type
def: "organisms living in a specific kind of environment" []
relationship: usually_has_external_link_to M0004 ! external_definition
relationship: ideally_has_external_link_to M0005 ! external_enumeration
is_a: GC0004 ! location_group_type

[Term]
id: GH0001
name: nutrients_level_requirement
namespace: group_type
def: "organisms which require a given quantitive level of availability of
     nutrients" []
comment: e.g. oligotrophic, copiotrophic
is_a: GC0002 ! habitat_requirement_type

[Term]
id: GH0002
name: specific_nutrient_availability
namespace: group_type
def: "organisms by their requirement of availability of a specific nutrient" []
is_a: GC0002 ! habitat_requirement_type

[Term]
id: GH0003
name: O2_requirement
namespace: group_type
def: "organisms by requirement of molecular oxygen level in their habitat" []
is_a: GC0002 ! habitat_requirement_type

[Term]
id: GH0004
name: salinity_requirement
namespace: group_type
def: "organisms by requirement of a salinity level in their habitats" []
is_a: GC0002 ! habitat_requirement_type

[Term]
id: GH0005
name: pH_requirement
namespace: group_type
def: "organisms by requirement of a pH range in their habitats" []
is_a: GC0002 ! habitat_requirement_type

[Term]
id: GH0006
name: temperature_requirement
namespace: group_type
def: "organisms by requirement of a temperature range in their habitats" []
is_a: GC0002 ! habitat_requirement_type

[Term]
id: GP0001
name: biological_interaction
namespace: group_type
def: "organisms by kind of interaction (or lack thereof) with other organisms" []
is_a: GC0003 ! phenotype_group_type

[Term]
id: GP0002
name: taxis
namespace: group_type
def: "organisms by their tendency to move or orient towards or against
     a given stimulus" []
is_a: GC0003 ! phenotype_group_type

[Term]
id: GP0003
name: metabolic
namespace: group_type
def: "organisms sharing a specific trait of their metabolism" []
is_a: GC0003 ! phenotype_group_type

[Term]
id: GP0004
name: gram_stain
namespace: group_type
def: "organisms according to their reactivity to Gram stain" []
is_a: GC0003 ! phenotype_group_type

[Term]
id: GP0005
name: trophic_strategy
namespace: group_type
def: "organisms which share the same strategy for obtaining energy and/or
     organic compounds" []
is_a: GC0003 ! phenotype_group_type

[Term]
id: GP0006
name: cultiviability
namespace: group_type
def: "organisms by the ability to cultivate them in a laboratory" []
is_a: GC0003 ! phenotype_group_type

[Term]
id: GP0007
name: resultive_disease_symptom
namespace: group_type
def: "patogenic organisms by the kind of disease or symptom that they
     cause (or lack thereof)" []
is_a: GC0003 ! phenotype_group_type

[Term]
id: GX0001
name: combined_group
namespace: group_type
def: "organisms which share or lack a number of conditions, which are described
     in other terms, and hereby combined by the set operations union and
     intersection" []
is_a: GC0005 ! derived_group_type
relationship: defined_by M0002 ! groups_combination_expression

[Term]
id: GX0002
name: inverted_group
namespace: group_type
def: "organisms which is not an instance of a specified group" []
is_a: GC0005 ! derived_group_type
relationship: defined_by M0011 ! group_inversion_expression
